Changed the types - output is a state

michael_formal/types.thy
@@ -1,20 +1,20 @@
 theory types
-  imports "~~/src/HOL/IMP/Hoare"
+  imports "~~/src/HOL/IMP/Hoare" "Show.Show_Instances"
 begin
 type_synonym label = string
 type_synonym arity = nat
-type_synonym inputs = state
+type_synonym inputs = "int list"
 type_synonym registers = state
 type_synonym outputs = state
 type_synonym guard = "bexp list"
 type_synonym output_function = "(string \<times> aexp) list"
 type_synonym update_function = "(string \<times> aexp) list"
 type_synonym statename = int
-type_synonym trace = "(label \<times> state) list" (*Ideally written as label(i1, i2, ...)*)
+type_synonym trace = "(label \<times> inputs) list" (*Ideally written as label(i1, i2, ...)*)
 type_synonym observation = "outputs list"
 
 
-record transition = 
+record transition =
   Label :: label
   Arity :: arity
   Guard :: guard
@@ -37,5 +37,27 @@ lemma "\<forall>z. \<exists>x y. (aval (V v) (join x y) = aval (V v) z)"
 
 lemma "\<forall> x y. \<exists>z. (aval (V v) z) = aval (V v) (join x y)"
   by auto
+
+definition index :: "int \<Rightarrow> string" where
+  "index i = ''i''@(showsp_int (nat i) i '''')"
+declare index_def [simp]
+
+lemma i1: "index 2 = ''i2''"
+  apply (simp add: showsp_int_def)
+  apply (simp add: showsp_nat.simps)
+  apply (simp add: shows_string_def)
+  done
+
+primrec input2state :: "int list \<Rightarrow> int \<Rightarrow> state" where
+  "input2state [] _ = <>" |
+  "input2state (h#t) i = (\<lambda>x. if x = (index i) then h else ((input2state t (i+1)) x))"
+declare input2state_def [simp]
+
+lemma "input2state [1, 2] 1 = <''i1'':=1, ''i2'':=2>"
+  apply (rule ext)
+  apply (simp add: showsp_int_def cong: if_cong)
+  apply (simp add: showsp_nat.simps)
+  apply (simp add: shows_string_def)
+  done
 
 end
